syn typed sec chan

theories/prob_eff_lang/probblaze/examples/DH_KE/advantage_schan.v
@@ -2,7 +2,7 @@ From clutch.prob_eff_lang.probblaze Require Import advantage.
 From iris.algebra Require Import excl.
 From iris.algebra.lib Require Import dfrac_agree.
 From clutch.prob_eff_lang.probblaze Require Import sem_def sem_types sem_judgement sem_row syntax semantics proofmode valgroup.
-From clutch.prob_eff_lang.probblaze Require Import xor sec_channel_def sec_channel_prf adequacy.
+From clutch.prob_eff_lang.probblaze Require Import xor sec_channel_def sec_channel_prf adequacy types interp fundamental.
 
 Import fingroup.
 Import fingroup.fingroup.
@@ -34,6 +34,32 @@ Section adv_schan.
       :=  (∀ᵣ θ__L ,(∀ᵣ θₕ, (((𝔾 -{ θₕ }-> 𝟙) × (𝟙 -{ θₕ }-> (Option  𝔾))) -{ sem_row_union  θₕ θ__L }-∘ 𝟙)) ⊸ (*type of client*)
                  (∀ᵣ θ₁, ∀ᵣ θ₂,  (((𝔾 × (𝟙 + 𝟙)) -{ θ₁ }-> 𝟙) × ((𝟙 + 𝟙) -{ θ₁ }-> Option 𝟙)) ⊸ (((𝟙 + 𝟙) -{ θ₂ }-> 𝟙) × ((𝟙 + 𝟙) -{ θ₂ }-> Option 𝟙)) -{ sem_row_union θ₁ (sem_row_union θ₂ θ__L) }-∘ 𝟙))%T.
 
+  Definition T_CHAN : type :=
+    (∀R: (∀R: ((τG -{ RVar 0%nat }-> ()) * (() -{ RVar 0%nat }-> (() + τG)) -{ RVar 0%nat ∪ᵣ (RVar 1%nat) }-∘ ())) -∘
+  (∀R: (∀R: (((τG * (() + ())) -{ RVar 1%nat }-> ()) * ((() + ()) -{ RVar 1%nat }-> (() + ()))) 
+            -∘ ((() + ()) -{ RVar 0%nat }-> ()) * ((() + ()) -{ RVar 0%nat }-> (() + ())) 
+                -{ RVar 1%nat ∪ᵣ (RVar 0%nat ∪ᵣ RVar 2%nat) }-∘ ()))).
+
+  Lemma T_CHAN_interp `{!probblazeRGS Σ} η μ δ ξ :
+    interp._ty η μ δ (T_CHAN ⇾ TBool) ξ = (τ_CHAN → 𝔹)%T.
+  Proof using All.
+    (* Only the group leaves are non-definitional; [HG] bridges them via
+       [τG_lrel] (instance supplied by the section's [G]). *)
+    assert (HG : ∀ ζ, interp._ty η μ δ τG ζ = sem_ty_group) by
+      (intros ζ; extensionality v1; extensionality v2; symmetry;
+       apply (τG_lrel (clutch_group := G _ _))).
+    rewrite /T_CHAN /τ_CHAN /sem_ty_option. simpl.
+    repeat f_equiv; first done.
+    apply functional_extensionality; intros?.
+    repeat f_equiv; first done.
+    - apply functional_extensionality; intros?.
+      rewrite HG. done.
+    - apply functional_extensionality; intros?.
+      f_equiv.
+      apply functional_extensionality; intros?.
+      rewrite HG. done.
+  Qed. 
+  
   Lemma adv_SCHAN A :
     (∀ `{!probblazeRGS Σ}, 
        ⊢ sem_val_typed A A (τ_CHAN → 𝔹)%T) →
@@ -42,6 +68,20 @@ Section adv_schan.
     intros. eapply sem_typed_advantage; eauto. split.
     - intros Hrgs. by unshelve eapply R_I_SCHAN.
     - intros Hrgs. by unshelve eapply I_R_SCHAN.
+  Qed. 
+
+  Lemma adv_SCHAN_typed A :
+   ⊢ᵥ A : (T_CHAN ⇾ TBool) →
+   nonneg (advantage A (R_CHAN xor_struct) (λ: "f", CHAN_SIM_lazy (F_CHAN "f"))%V #true) = 0%R.
+  Proof using All.
+    intros HAtyped. apply adv_SCHAN. 
+    intros HRGS.
+    apply (@fundamental_val Σ HRGS) in HAtyped.
+    iPoseProof HAtyped as "Hadv".
+    unfold bin_log_val_related.
+    iSpecialize ("Hadv" $! [] [] ∅ []). 
+    repeat rewrite ?interp_TArrow ?interp_TBang.
+    by rewrite T_CHAN_interp.
   Qed. 
   
 End adv_schan.
